state/Witnessable.fst
@@ -16,40 +16,37 @@ class witnessable (t:Type) = {
   satisfy_on_heap_monotonic : x:t -> pred:mref_heap_stable_pred -> h0:heap -> h1:heap ->
     Lemma (requires (h0 `heap_rel` h1 /\ satisfy_on_heap x h0 pred))
           (ensures (satisfy_on_heap x h1 pred));
-
-  pwitness : x:t -> pred:mref_heap_stable_pred -> ST (precall:(unit -> ST unit (fun _ -> True) (fun h0 _ h1 -> h0 == h1 /\ satisfy_on_heap x h1 pred)))
-    (requires (fun h0 -> satisfy_on_heap x h0 pred))
-    (ensures (fun h0 _ h1 -> h0 == h1));
 }
+
+// let __satisfy_on_heap #t {| c:witnessable t |} x h (pred:mref_heap_pred) = 
+//   c.satisfy x (fun #a #rel r -> pred r h)
+
+// let __satisfy_on_heap_monotonic #t {| c:witnessable t |} (x:t) (pred:mref_heap_stable_pred) h0 h1 :
+//   Lemma (requires (h0 `heap_rel` h1 /\ __satisfy_on_heap x h0 pred))
+//         (ensures (__satisfy_on_heap x h1 pred)) = ()
 
 instance witnessable_mref (t:Type) (rel:FStar.Preorder.preorder t) {| c:witnessable t |} : witnessable (mref t rel) = {
   satisfy = (fun x pred -> pred x);
   satisfy_on_heap = (fun x h pred -> pred x h);
   satisfy_on_heap_monotonic = (fun x pred h0 h1 -> ());
-  pwitness = (fun x pred ->
-    MST.Tot.witness (pred x);
-    (fun () -> MST.Tot.recall (pred x)))
 }
 
 instance witnessable_unit : witnessable unit = {
   satisfy = (fun _ _ -> True);
   satisfy_on_heap = (fun _ _ _ -> True);
   satisfy_on_heap_monotonic = (fun _ _ _ _ -> ());
-  pwitness = (fun _ _ -> (fun () -> ()));
 }
 
 instance witnessable_int : witnessable int = {
   satisfy = (fun _ _ -> True);
   satisfy_on_heap = (fun _ _ _ -> True);
   satisfy_on_heap_monotonic = (fun _ _ _ _ -> ());
-  pwitness = (fun _ _ -> (fun () -> ()));
 }
 
 instance witnessable_refinement (t:Type) {| c:witnessable t |} (p:t -> Type0) : witnessable (x:t{p x}) = {
   satisfy = (fun (x:t{p x}) pred -> c.satisfy x pred);
   satisfy_on_heap = (fun (x:t{p x}) h pred -> c.satisfy_on_heap x h pred);
   satisfy_on_heap_monotonic = (fun (x:t{p x}) pred h0 h1 -> c.satisfy_on_heap_monotonic x pred h0 h1);
-  pwitness = (fun (x:t{p x}) pred -> c.pwitness x pred)
 }
 
 instance witnessable_arrow
@@ -60,7 +57,6 @@ instance witnessable_arrow
   satisfy = (fun _ _ -> True);
   satisfy_on_heap = (fun _ _ _ -> True);
   satisfy_on_heap_monotonic = (fun _ _ _ _ -> ());
-  pwitness = (fun _ _ -> (fun () -> ()));
 }
 
 instance witnessable_option (t:Type) {| c:witnessable t |} : witnessable (option t) = {
@@ -75,13 +71,7 @@ instance witnessable_option (t:Type) {| c:witnessable t |} : witnessable (option
   satisfy_on_heap_monotonic = (fun x pred h0 h1 ->
     match x with
     | None -> ()
-    | Some x' -> c.satisfy_on_heap_monotonic x' pred h0 h1);
-  pwitness = (fun x pred ->
-    match x with
-    | None -> (fun () -> ())
-    | Some x' ->
-      let w = c.pwitness x' pred in (fun () -> w ()))
-}
+    | Some x' -> c.satisfy_on_heap_monotonic x' pred h0 h1);}
 
 instance witnessable_pair (t1:Type) (t2:Type) {| c1:witnessable t1 |} {| c2:witnessable t2 |} : witnessable (t1 * t2) = {
   satisfy = (fun (x1, x2) pred -> c1.satisfy x1 pred /\ c2.satisfy x2 pred);
@@ -89,10 +79,6 @@ instance witnessable_pair (t1:Type) (t2:Type) {| c1:witnessable t1 |} {| c2:witn
   satisfy_on_heap_monotonic = (fun (x1, x2) pred h0 h1 ->
     c1.satisfy_on_heap_monotonic x1 pred h0 h1;
     c2.satisfy_on_heap_monotonic x2 pred h0 h1);
-  pwitness = (fun (x1, x2) pred ->
-    let w1 = c1.pwitness x1 pred in
-    let w2 = c2.pwitness x2 pred in
-    (fun () -> w1 (); w2 ()))
 }
 
 instance witnessable_sum (t1:Type) (t2:Type) {| c1:witnessable t1 |} {| c2:witnessable t2 |} : witnessable (either t1 t2) = {
@@ -108,10 +94,6 @@ instance witnessable_sum (t1:Type) (t2:Type) {| c1:witnessable t1 |} {| c2:witne
     match x with
     | Inl x1 -> c1.satisfy_on_heap_monotonic x1 pred h0 h1
     | Inr x2 -> c2.satisfy_on_heap_monotonic x2 pred h0 h1);
-  pwitness = (fun x pred ->
-    match x with
-    | Inl x1 -> (let w = c1.pwitness x1 pred in (fun () -> w ()))
-    | Inr x2 -> (let w = c2.pwitness x2 pred in (fun () -> w ())))
 }
 
 let rec forall_in_list (l:list 'a) (pred:'a -> Type0) : Type0 =
@@ -137,8 +119,6 @@ instance witnessable_list (t:Type) {| c:witnessable t |} : witnessable (list t) 
 
   satisfy_on_heap_monotonic = (fun l pred h0 h1 ->
     list_satisfy_on_heap_monotonic l pred h0 h1);
-
-  pwitness = (fun l pred -> admit ());
 }
 
 
@@ -158,20 +138,10 @@ instance witnessable_llist (t:Type) {| c:witnessable t |} : witnessable (linkedL
     | LLNil -> ()
     | LLCons x xsref -> c.satisfy_on_heap_monotonic x pred h0 h1
   );
-
-  pwitness = (fun l pred ->
-    match l with
-    | LLNil -> (fun () -> ())
-    | LLCons x xsref ->
-      let w = c.pwitness x pred in
-      MST.Tot.witness (pred xsref);
-      (fun () -> w (); MST.Tot.recall (pred xsref))
-  );
 }
 
 instance witnessable_univ_raise (t:Type u#a) {| c:witnessable t |} : witnessable (raise_t u#a u#b t) = {
   satisfy = (fun x -> c.satisfy (downgrade_val x));
   satisfy_on_heap = (fun x -> c.satisfy_on_heap (downgrade_val x));
   satisfy_on_heap_monotonic = (fun x -> c.satisfy_on_heap_monotonic (downgrade_val x));
-  pwitness = (fun x -> c.pwitness (downgrade_val x));
 }
